polyvec_compress_1 proofs

proof/correctness/avx2/KyberPolyvec_avx2_prevec.ec
@@ -1,6 +1,6 @@
 require import AllCore List Int IntDiv CoreMap.
 from Jasmin require import JModel.
-require import Array16 Array32 Array128 Array256 Array400 Array768.
+require import Array4 Array16 Array32 Array128 Array256 Array400 Array768 Array960.
 require import WArray32 WArray256 WArray512 WArray800 WArray1536 WArray168 WArray800.
 require import AVX2_Ops.
 require import Jkem_avx2.
@@ -104,6 +104,81 @@ module Mprevec = {
          (fun i => if (2 * 256) <= i < (2 * 256) + 256 then aux.[i-(2 * 256)]
          else a.[i]);
     return ();
+  }
+
+  proc polyvec_compress_1 (rp:W8.t Array960.t, a:W16.t Array768.t) : W8.t Array960.t = {
+    var aux: int;
+
+    var v:t16u16;
+    var v8:t16u16;
+    var off:t16u16;
+    var shift1:t16u16;
+    var mask:t16u16;
+    var shift2:t16u16;
+    var shift2_q:t4u64;
+    var sllvdidx:t8u32;
+    var sllvdidx_q:t4u64;
+    var shufbidx:t32u8;
+    var i:int;
+    var f0:t16u16;
+    var f1:t16u16;
+    var f2:t16u16;
+    var t0:t16u8;
+    var t1:t16u8;
+    var f0_b:t32u8;
+    var f0_d:t8u32;
+    var f0_q:t4u64;
+    var t0_d:t4u8;
+
+    a <@ polyvec_csubq (a);
+
+    v <- jvx16;
+    v8 <@ Ops.iVPSLL_16u16(v, (W8.of_int 3));
+    off <@ Ops.iVPBROADCAST_16u16(pvc_off_s);
+    shift1 <@ Ops.iVPBROADCAST_16u16(pvc_shift1_s);
+    mask <@ Ops.iVPBROADCAST_16u16(pvc_mask_s);
+    shift2_q <@ Ops.iVPBROADCAST_4u64(pvc_shift2_s);
+    shift2 <- f4u64_t16u16 shift2_q;
+    sllvdidx_q <@ Ops.iVPBROADCAST_4u64(pvc_sllvdidx_s);
+    sllvdidx <- f4u64_t8u32 sllvdidx_q;
+    shufbidx <- pvc_shufbidx_s;
+
+    aux <- ((3 * 256) %/ 16);
+    i <- 0;
+
+    while (i < aux) {
+      f0 <- Array16.init (fun j => a.[16 * i + j]);
+      f1 <@ Ops.iVPMULL_16u16(f0, v8);
+      f2 <@ Ops.iVPADD_16u16(f0, off);
+      f0 <@ Ops.iVPSLL_16u16(f0, (W8.of_int 3));
+      f0 <@ Ops.iVPMULH_256(f0, v);
+      f2 <@ Ops.iVPSUB_16u16(f1, f2);
+      f1 <@ Ops.iVPANDN_16u16(f1, f2);
+      f1 <@ Ops.iVPSRL_16u16(f1, (W8.of_int 15));
+      f0 <@ Ops.iVPSUB_16u16(f0, f1);
+      f0 <@ Ops.iVPMULHRS_256(f0, shift1);
+      f0 <@ Ops.iVPAND_16u16(f0, mask);
+      f0_d <@ Ops.iVPMADDWD_256(f0, shift2);
+
+      f0_d <@ Ops.iVPSLLV_8u32(f0_d, sllvdidx);
+
+      f0_q <- f8u32_t4u64 f0_d;
+      f0_q <@ Ops.iVPSRL_4u64(f0_q, (W8.of_int 12));
+
+      f0_b <- f4u64_t32u8 f0_q;
+      f0_b <@ Ops.iVPSHUFB_256(f0_b, shufbidx);
+
+      f0 <- f32u8_t16u16 f0_b;
+      t0 <@ Ops.itruncate_16u16_8u16(f0);
+      t1 <@ Ops.iVEXTRACTI128_16u8(f0, (W8.of_int 1));
+      t0 <@ Ops.iVPBLENDW_128_16u8(t0, t1, (W8.of_int 224));
+
+      rp <- Array960.fill (fun j => t0.[j %% 20]) (20*i) 16 rp;
+      t0_d <@ Ops.iVPEXTR_32(t1, (W8.of_int 0));
+      rp <- Array960.fill (fun j => t0_d.[j %% 4]) (20*i + 16) 4 rp;
+      i <- i + 1;
+    }
+    return (rp);
   }
 
   proc polyvec_compress (rp:W64.t, a:W16.t Array768.t) : unit = {
